cache stuff

concurrency/scache/CacheSM.i.dfy
@@ -4,13 +4,15 @@ include "../../lib/Base/Option.s.dfy"
 
 module CacheSSM refines DiskSSM(CacheIfc) {
   import opened Options
+  import CacheIfc
 
-  datatype Status = Empty | Reading | Clean | Dirty | Writeback
+  datatype Status = //Empty | Reading |
+        Clean | Dirty | Writeback
 
-  datatype Entry = Entry(
-    disk_idx: nat, // meaningless if Status == Empty
-    data: DiskIfc.Block // meaningless if Status in {Empty, Reading}
-  )
+  datatype Entry =
+    | Empty
+    | Reading(disk_idx: nat)
+    | Entry(disk_idx: nat, data: DiskIfc.Block)
 
   // Notes:
   //
@@ -86,33 +88,45 @@ module CacheSSM refines DiskSSM(CacheIfc) {
       map[], map[], {}, {}, map[], map[], map[], map[])
   }
 
+  function CacheReading(cache_idx: nat, disk_idx: nat) : M {
+    M(map[],
+      map[cache_idx := Reading(disk_idx)],
+      map[], map[], {}, {}, map[], map[], map[], map[])
+  }
+
+  function CacheEmpty(cache_idx: nat) : M {
+    M(map[],
+      map[cache_idx := Empty],
+      map[], map[], {}, {}, map[], map[], map[], map[])
+  }
+
   function CacheStatus(cache_idx: nat, status: Status) : M {
     M(map[], map[],
       map[cache_idx := status],
       map[], {}, {}, map[], map[], map[], map[])
   }
 
-  function WriteReq(disk_idx: nat, data: DiskIfc.Block) : M {
+  function DiskWriteReq(disk_addr: nat, data: DiskIfc.Block) : M {
     M(map[], map[], map[],
-      map[disk_idx := data],
+      map[disk_addr := data],
       {}, {}, map[], map[], map[], map[])
   }
 
-  function WriteResp(disk_idx: nat) : M {
+  function DiskWriteResp(disk_addr: nat) : M {
     M(map[], map[], map[], map[],
-      {disk_idx},
+      {disk_addr},
       {}, map[], map[], map[], map[])
   }
 
-  function ReadReq(disk_idx: nat) : M {
+  function DiskReadReq(disk_addr: nat) : M {
     M(map[], map[], map[], map[], {},
-      {disk_idx},
+      {disk_addr},
       map[], map[], map[], map[])
   }
 
-  function ReadResp(disk_idx: nat, data: DiskIfc.Block) : M {
+  function DiskReadResp(disk_addr: nat, data: DiskIfc.Block) : M {
     M(map[], map[], map[], map[], {}, {},
-      map[disk_idx := data],
+      map[disk_addr := data],
       map[], map[], map[])
   }
 
@@ -161,12 +175,6 @@ module CacheSSM refines DiskSSM(CacheIfc) {
       {}
   }
 
-  function DiskWriteReq(disk_addr: nat, data: DiskIfc.Block) : M
-  function DiskWriteResp(disk_addr: nat) : M
-
-  function DiskReadReq(disk_addr: nat) : M
-  function DiskReadResp(disk_addr: nat, data: DiskIfc.Block) : M
-
   predicate Init(s: M)
 
   function dot3(a: M, b: M, c: M) : M {
@@ -178,26 +186,23 @@ module CacheSSM refines DiskSSM(CacheIfc) {
   }
 
   predicate StartRead(shard: M, shard': M,
-      cache_idx: nat, disk_idx: nat, junk_data: DiskIfc.Block, junk_disk_idx: nat) {
-    && shard == dot3(
-        CacheStatus(cache_idx, Empty),
-        CacheEntry(cache_idx, junk_disk_idx, junk_data),
+      cache_idx: nat, disk_idx: nat) {
+    && shard == dot(
+        CacheEmpty(cache_idx),
         DiskIdxToCacheIdx(disk_idx, None)
        )
-    && shard' == dot4(
-        CacheStatus(cache_idx, Reading),
-        CacheEntry(cache_idx, disk_idx, junk_data),
+    && shard' == dot3(
+        CacheReading(cache_idx, disk_idx),
         DiskIdxToCacheIdx(disk_idx, Some(cache_idx)),
-        ReadReq(disk_idx)
+        DiskReadReq(disk_idx)
        )
   }
 
   predicate FinishRead(shard: M, shard': M,
-      cache_idx: nat, disk_idx: nat, junk_data: DiskIfc.Block, data: DiskIfc.Block) {
-    && shard == dot3(
-        CacheStatus(cache_idx, Reading),
-        CacheEntry(cache_idx, disk_idx, junk_data),
-        ReadResp(disk_idx, data)
+      cache_idx: nat, disk_idx: nat, data: DiskIfc.Block) {
+    && shard == dot(
+        CacheReading(cache_idx, disk_idx),
+        DiskReadResp(disk_idx, data)
        )
     && shard' == dot(
         CacheStatus(cache_idx, Clean),
@@ -214,7 +219,7 @@ module CacheSSM refines DiskSSM(CacheIfc) {
     && shard' == dot3(
         CacheStatus(cache_idx, Writeback),
         CacheEntry(cache_idx, disk_idx, data), // unchanged
-        WriteReq(disk_idx, data)
+        DiskWriteReq(disk_idx, data)
        )
   }
 
@@ -223,7 +228,7 @@ module CacheSSM refines DiskSSM(CacheIfc) {
     && shard == dot3(
         CacheEntry(cache_idx, disk_idx, data),
         CacheStatus(cache_idx, Writeback),
-        WriteResp(disk_idx)
+        DiskWriteResp(disk_idx)
        )
     && shard' == dot(
         CacheEntry(cache_idx, disk_idx, data), // unchanged
@@ -238,11 +243,52 @@ module CacheSSM refines DiskSSM(CacheIfc) {
         CacheEntry(cache_idx, disk_idx, data),
         DiskIdxToCacheIdx(disk_idx, cache_idx2)
       )
-    && shard == dot3(
-        CacheStatus(cache_idx, Empty),
-        CacheEntry(cache_idx, disk_idx, data),
+    && shard == dot(
+        CacheEmpty(cache_idx),
         DiskIdxToCacheIdx(disk_idx, None)
       )
+  }
+
+  predicate ObserveCleanForSync(shard: M, shard': M,
+    cache_idx: nat, disk_idx: nat, data: DiskIfc.Block, rid: RequestId, s: set<nat>)
+  {
+    && shard == dot3(
+      CacheStatus(cache_idx, Clean),
+      CacheEntry(cache_idx, disk_idx, data),
+      SyncReq(rid, s)
+    )
+    && shard' == dot3(
+      CacheStatus(cache_idx, Clean),
+      CacheEntry(cache_idx, disk_idx, data),
+      SyncReq(rid, s - {disk_idx})
+    )
+  }
+
+  predicate ApplyRead(shard: M, shard': M,
+      cache_idx: nat, disk_idx: nat, data: DiskIfc.Block, rid: RequestId)
+  {
+    && shard == dot(
+      CacheEntry(cache_idx, disk_idx, data),
+      NormalTicket(rid, CacheIfc.ReadInput(disk_idx))
+    )
+    && shard' == dot(
+      CacheEntry(cache_idx, disk_idx, data),
+      NormalStub(rid, CacheIfc.ReadOutput(data))
+    )
+  }
+
+  predicate ApplyWrite(shard: M, shard': M,
+      cache_idx: nat, disk_idx: nat, data: DiskIfc.Block, new_data: DiskIfc.Block,
+      rid: RequestId)
+  {
+    && shard == dot(
+      CacheEntry(cache_idx, disk_idx, data),
+      NormalTicket(rid, CacheIfc.WriteInput(disk_idx, new_data))
+    )
+    && shard' == dot(
+      CacheEntry(cache_idx, disk_idx, new_data),
+      NormalStub(rid, CacheIfc.WriteOutput)
+    )
   }
 
   predicate Internal(shard: M, shard': M)
@@ -251,46 +297,73 @@ module CacheSSM refines DiskSSM(CacheIfc) {
     true
   }
 
-/*
   lemma InitImpliesInv(s: M)
-  requires Init(s)
+  //requires Init(s)
   ensures Inv(s)
+  {
+  }
 
   lemma InternalPreservesInv(shard: M, shard': M, rest: M)
-  requires Inv(dot(shard, rest))
-  requires Internal(shard, shard')
+  //requires Inv(dot(shard, rest))
+  //requires Internal(shard, shard')
   ensures Inv(dot(shard', rest))
+  {
+  }
 
   lemma NewTicketPreservesInv(whole: M, whole': M, rid: RequestId, input: IOIfc.Input)
-  requires Inv(whole)
-  requires NewTicket(whole, whole', rid, input)
+  //requires Inv(whole)
+  //requires NewTicket(whole, whole', rid, input)
   ensures Inv(whole')
+  {
+  }
 
   lemma ConsumeStubPreservesInv(whole: M, whole': M, rid: RequestId, output: IOIfc.Output)
-  requires Inv(whole)
-  requires ConsumeStub(whole, whole', rid, output)
+  //requires Inv(whole)
+  //requires ConsumeStub(whole, whole', rid, output)
   ensures Inv(whole')
+  {
+  }
 
   lemma ProcessReadPreservesInv(disk_addr: nat, data: DiskIfc.Block, rest: M)
-  requires Inv(dot(DiskReadReq(disk_addr, |data|), rest))
+  //requires Inv(dot(DiskReadReq(disk_addr, |data|), rest))
   ensures Inv(dot(DiskReadResp(disk_addr, data), rest))
+  {
+  }
 
   lemma ProcessWritePreservesInv(disk_addr: nat, data: DiskIfc.Block, rest: M)
-  requires Inv(dot(DiskWriteReq(disk_addr, data), rest))
-  ensures Inv(dot(DiskWriteResp(disk_addr, |data|), rest))
+  //requires Inv(dot(DiskWriteReq(disk_addr, data), rest))
+  ensures Inv(dot(DiskWriteResp(disk_addr), rest))
+  {
+  }
 
   lemma dot_unit(x: M)
   ensures dot(x, unit()) == x
+  {
+  }
 
   lemma commutative(x: M, y: M)
   ensures dot(x, y) == dot(y, x)
+  {
+    if dot(x,y) == Fail {
+      assert dot(x, y) == dot(y, x);
+    } else {
+      assert dot(x, y) == dot(y, x);
+    }
+  }
 
   lemma associative(x: M, y: M, z: M)
   ensures dot(x, dot(y, z)) == dot(dot(x, y), z)
+  {
+    if dot(x, dot(y, z)) == Fail {
+      assert dot(x, dot(y, z)) == dot(dot(x, y), z);
+    } else {
+      assert dot(x, dot(y, z)) == dot(dot(x, y), z);
+    }
+  }
 
   lemma exists_inv_state()
   returns (s: M)
   ensures Inv(s)
-
-*/
+  {
+  }
 }
